trunk/color/ProofChecker/Proof.v
@@ -1,0 +1,39 @@
+(**
+CoLoR, a Coq library on rewriting and termination.
+See the COPYRIGHTS and LICENSE files.
+
+- Adam Koprowski, 2009-03-24
+
+A specification of termination proofs.
+*)
+
+Set Implicit Arguments.
+
+Require Import ZArith.
+Require Import List.
+Require Import ASignature.
+
+Section Proof.
+
+Variable Sig : Signature.
+
+(** [trsInt si] is a representation for an interpretation assigning type 
+    [si] to a function symbol. It is represented by a list of pairs: 
+    [(f, fi)], where [f] is a function symbol and [fi] is its 
+    interpretation. *)
+Definition trsInt symInt := list (Sig * symInt).
+
+(** [monomial] is a monomial in representation of a polynomial. 
+    A monomial [C * x_0^i_0 * ... * x_n^i_n] is represented as:
+    [(C, i_0::...::i_n)]. *)
+Definition monomial := (Z * list nat)%type.
+
+(** [polynomial] is a list of monomials so [m_0 + ... + m_n] becomes 
+    [m_0::...::m_n]. *)
+Definition polynomial := list monomial.
+
+Inductive TerminationProof :=
+| TP_PolyInt (PI: trsInt polynomial) (Prf : TerminationProof)
+| TP_ProblemEmpty.
+
+End Proof.
