trunk/color/Term/WithArity/MonAlgChecker.v
@@ -1,0 +1,296 @@
+(**
+CoLoR, a Coq library on rewriting and termination.
+See the COPYRIGHTS and LICENSE files.
+
+- Adam Koprowski, 2009-03-25
+
+  This file contains a proof checker for termination criteria based
+on (extended) weakly monotone algebra.
+*)
+
+Require Import ATrs.
+Require Import RelUtil.
+Require Import SN.
+Require Import AWFMInterpretation.
+Require Import AMannaNess.
+Require Import ACompat.
+Require Import RelMidex.
+Require Import ListUtil.
+Require Import ListForall.
+Require Import ARelation.
+Require Import LogicUtil.
+Require Import ExcUtil.
+Require Import IntBasedChecker.
+Require Import Problem.
+Require Import Program.
+Require Import NaryFunction.
+Require Import Proof.
+
+Set Implicit Arguments.
+
+Section MonAlgChecker.
+
+Variable Sig : Signature.
+
+Notation Problem := (Problem Sig).
+Notation term := (term Sig).
+Notation rule := (@rule Sig).
+Notation rules := (@list rule).
+
+Variable domain : Type.
+Let D := domain.
+Variable domain_elt : D.
+
+Variable succ : relation D.
+Variable succeq : relation D.
+Variable succ_wf : WF succ.
+Variable succ_succeq_compat : absorb succ succeq.
+
+Variable arSymInt : nat -> Set.
+Notation symInt := (symInt Sig arSymInt).
+Notation funInt := (funInt Sig arSymInt).
+
+Variable defaultInt : forall n, arSymInt n.
+
+Variable interpret : forall n, arSymInt n -> naryFunction domain n.
+
+Program Definition makeI (int : forall f, funInt f) :=
+  mkInterpretation (Sig:=Sig) domain_elt (fun f => interpret (int f)).
+
+Variable check_succ : forall i r, Exc (IR (makeI i) succ (lhs r) (rhs r)).
+Variable check_succeq : forall i r, Exc (IR (makeI i) succeq (lhs r) (rhs r)).
+
+Section given_int.
+
+Variable i : forall f, funInt f.
+Notation I := (makeI i).
+
+Notation IR_succ := (IR I succ).
+Notation IR_succeq := (IR I succeq).
+
+Section reduction_pairs.
+
+Variable wm : monotone I succeq.
+
+Lemma wf_IR_succ : WF IR_succ.
+
+Proof.
+  intros. apply IR_WF. apply succ_wf.
+Qed.
+
+Lemma absorb_succ_succeq : absorb IR_succ IR_succeq.
+
+Proof.
+  intros x z xz val.
+  apply succ_succeq_compat.
+  destruct xz as [y [ge_xy gt_yz]].
+  exists (term_int val y). split; auto.
+Qed.
+
+Definition wrp := mkWeak_reduction_pair 
+  (IR_substitution_closed (I:=I) (R:=succ))
+  (IR_substitution_closed (I:=I) (R:=succeq))
+  (IR_context_closed wm) absorb_succ_succeq wf_IR_succ.
+
+Section sm.
+
+Variable sm : monotone I succ.
+
+Definition rp := mkReduction_pair 
+  (IR_substitution_closed (I:=I) (R:=succ))
+  (IR_substitution_closed (I:=I) (R:=succeq))
+  (IR_context_closed sm) (IR_context_closed wm)
+  absorb_succ_succeq wf_IR_succ.
+
+End sm.
+
+End reduction_pairs.
+
+Section prover.
+
+Variable check_int_wm : Exc (monotone I succeq).
+Variable check_int_sm : Exc (monotone I succeq /\ monotone I succ).
+
+Program Definition check_compat (R : rules) (F : relation D)
+  (check_compat : forall i r, Exc (IR (makeI i) F (lhs r) (rhs r))) :
+  Exc (compat (IR (makeI i) F) R) :=
+  match lforall_exc _ (check_compat i) R with
+  | value _ => value _
+  | error => error
+  end. 
+
+Next Obligation.
+Proof with try discriminate; auto.
+  destruct_call lforall_exc...
+  intros t u Rtu. destruct (lforall_in wildcard' Rtu). hyp.
+Qed.
+
+Program Definition simplify (R : rules) : 
+  Exc { Rge : rules  | 
+          exists Rgt : rules,
+            compat IR_succ Rgt /\ 
+            compat IR_succeq Rge /\
+            incl R (Rgt ++ Rge)
+      } := 
+  let (Rp, obl) := partition_exc _ (check_succ i) R in
+    match check_compat (snd Rp) check_succeq with
+    | error => error
+    | value _ => value (snd Rp)
+    end.
+
+Next Obligation.
+Proof with try discriminate; auto.
+  exists l. destruct_call check_compat...
+  repeat split...
+  intros t u Rtu. exact (lforall_in H Rtu).
+  intros p pR. apply in_or_app. apply H1...
+Qed.
+
+Program Definition applyMonotoneAlgebra (P : Problem) : 
+  Exc { P' : Problem | Prob_WF P' -> Prob_WF P } :=
+
+  match P with
+  | FullTerm R =>
+      match check_int_sm with
+      | error => error
+      | value sm =>
+          match simplify R with
+          | error => error
+          | value R' => value (FullTerm R')
+          end
+      end
+  | RelTopTerm T R =>
+      match check_int_wm with
+      | error => error
+      | value wm =>
+        match check_compat T check_succeq with
+        | error => error
+        | value _ => 
+            match simplify R with
+            | error => error
+            | value R' => value (RelTopTerm T R')
+            end
+        end
+      end
+  | RelTerm T R =>
+      match check_int_sm with
+      | error => error
+      | value sm =>
+          match simplify T with
+          | error => error
+          | value T' =>
+              match simplify R with
+              | error => error
+              | value R' => value (RelTerm T' R')
+              end
+          end
+      end
+  end.
+
+Next Obligation.
+Proof with try discriminate; auto.
+  destruct_call simplify... 
+  clear Heq_anonymous0 s. decomp_hyps.
+  apply WF_incl with (red (x ++ R')). apply red_incl...
+  apply rule_elimination with (rp H1 H2)...
+Qed.
+Next Obligation.
+Proof with try discriminate; auto.
+  destruct_call simplify... 
+  clear Heq_anonymous0 Heq_anonymous1 s. decomp_hyps.
+  apply WF_incl with (hd_red_mod T (x ++ R')).
+  comp. apply hd_red_incl...
+  apply rule_elimination_hd_mod with (wrp wm)...
+Qed.
+Next Obligation.
+Proof with try discriminate; auto.
+  do 2 destruct_call simplify... 
+  clear Heq_anonymous0 Heq_anonymous1 s s0. decomp_hyps.
+  apply WF_incl with (red_mod (x0 ++ T') (x ++ R')).
+  comp. apply incl_rtc. apply red_incl... apply red_incl...
+  apply rule_elimination_mod with (rp H2 H3)...
+Qed.
+
+End prover.
+
+End given_int.
+
+Record monSpec monR := 
+  { monP : symInt -> Prop
+  ; mon_check : forall (i : symInt), Exc (monP i)
+  ; mon_ok : forall (i : symInt), 
+      monP i -> Vmonotone (interpret (projT2 i)) monR
+  }.
+
+Let buildSymInt := buildSymInt Sig arSymInt.
+Let defaultIntForSymbol := defaultIntForSymbol Sig arSymInt defaultInt.
+
+Variable wm : monSpec succeq.
+Variable sm : monSpec succ.
+Variable sm_imp_wm : forall s, monP sm s -> monP wm s.
+Variable sm_default : forall f, (monP sm) 
+  (buildSymInt (defaultIntForSymbol f)).
+
+Lemma wm_default : forall f,
+  (monP wm) (buildSymInt (defaultIntForSymbol f)).
+
+Proof with auto.
+  intros. apply sm_imp_wm...
+Qed.
+
+Section monotonicityChecker.
+
+Variable i : list symInt.
+Let I := (makeI (buildInt defaultInt i)).
+
+Let buildInt := (buildInt defaultInt i).
+
+Program Definition check_wm : Exc (monotone I succeq) :=
+  match @checkProp Sig arSymInt defaultInt (monP wm) (mon_check wm) wm_default i with
+  | error => error
+  | value _ => value _
+  end.
+
+Next Obligation.
+Proof with auto.
+  intro f. apply (mon_ok wm (buildSymInt (buildInt f))).
+  destruct_call checkProp... 
+Qed.
+
+Program Definition check_sm : 
+  Exc (monotone I succeq /\ monotone I succ) :=
+  match @checkProp Sig arSymInt defaultInt (monP sm) (mon_check sm) sm_default i with
+  | error => error
+  | value _ => value _
+  end.
+
+Next Obligation.
+Proof with auto.
+  split; intro f.
+  apply (mon_ok wm (buildSymInt (buildInt f))).
+  apply sm_imp_wm.
+  destruct_call checkProp...
+  apply (mon_ok sm (buildSymInt (buildInt f))).
+  destruct_call checkProp... 
+Qed.
+
+End monotonicityChecker.
+
+Section solver.
+
+Variable rawSymInt : Type.
+Variable rti : rawTrsInt Sig rawSymInt.
+Variable check_ri : Sig -> rawSymInt -> Exc symInt.
+
+Program Definition monotoneAlgebraSolver (P : Problem) :
+  Exc { P' : Problem | Prob_WF P' -> Prob_WF P } :=
+
+  match processInt check_ri rti with
+  | error => error
+  | value fis =>
+      applyMonotoneAlgebra (check_wm fis) (check_sm fis) P
+  end.
+
+End solver.
+
+End MonAlgChecker.
